add except and put requirements

Classes/Monad/MonadExcept.v
@@ -20,7 +20,7 @@ Arguments throw : simpl never.
 Arguments catch : simpl never.
 Hint Rewrite @throw_left @catch_left @catch_right @catch_return : monads.
 
-Class MonadExceptSound (M M' : Type → Type) 
+Class catch_op_sound (M M' : Type → Type) 
   {MM : Monad M} {MF : MonadExcept M}
   {MM' : Monad M'} {MF' : MonadExcept M'}
   {GM : ∀ A A', Galois A A' → Galois (M A) (M' A')} : Prop :=
@@ -32,3 +32,9 @@ Class MonadExceptSound (M M' : Type → Type)
     γ p2 p2' → 
     γ (catch p1 p2) (catch p1' p2').
 
+Class throw_op_sound (M M' : Type → Type) 
+  {MM : Monad M} {MF : MonadExcept M}
+  {MM' : Monad M'} {MF' : MonadExcept M'}
+  {GM : ∀ A A', Galois A A' → Galois (M A) (M' A')} : Prop :=
+  throw_sound : ∀ {A A'} {GA : Galois A A'},
+    γ (throw (A:=A)) (throw (A:=A')).
